kremlib/LowStar.Lib.LinkedList2.fst
@@ -1,12 +1,13 @@
 module LowStar.Lib.LinkedList2
 
-/// This module provides a convenient abstraction over LL1 which uses a ``v``
+/// This module provides a convenient abstraction over LL11 which uses a ``v``
 /// function, therefore eliminating a large amount of syntactic overhead. It
 /// also takes care of packing the existential, dealing with the extra outer
-/// reference, and suitable high-level operations.
+/// reference, and providing inclusion of the footprint in a static region at
+/// all times.
 ///
 /// Clients who want to modify the spine of the list or iterate over it can
-/// always use the LL1 definitions. AssocList is such an example.
+/// always use the LL11 definitions. AssocList is such an example.
 
 open LowStar.BufferOps
 
@@ -17,17 +18,17 @@ module L = FStar.List.Tot
 module U32 = FStar.UInt32
 module ST = FStar.HyperStack.ST
 
-module LL = LowStar.Lib.LinkedList
+module LL1 = LowStar.Lib.LinkedList
 
 open FStar.HyperStack.ST
 
 #set-options "--fuel 0 --ifuel 0"
 
 // Thanks to the KreMLin optimization, this type will extract just like
-// ``B.pointer (LL.t a)`` would, with no indirection due to the record.
+// ``B.pointer (LL1.t a)`` would, with no indirection due to the record.
 noeq
 type t a = {
-  ptr: B.pointer (LL.t a);
+  ptr: B.pointer (LL1.t a);
   // Relies on a new pointer-to-unit elimination phase in KreMLin
   v: B.pointer (G.erased (list a));
   // For separation; all erased.
@@ -44,23 +45,23 @@ let invariant #a h ll =
   // materializing the list at any time) to a ``v`` function which makes
   // specifications much easier. Any time the invariant holds, the pointer ``v``
   // holds a computationally-irrelevant representation of the list that in turns
-  // allows us to under-the-hood state the various predicates from LL that
+  // allows us to under-the-hood state the various predicates from LL1 that
   // require exhibiting a list.
   B.live h ll.ptr /\
   B.freeable ll.ptr /\
   B.live h ll.v /\
   B.freeable ll.v /\
-  LL.well_formed h head v /\
-  LL.invariant h head v /\
+  LL1.well_formed h head v /\
+  LL1.invariant h head v /\
 
   // We use regions for separation only, not for any footprint reasoning:
   // - ptr_v_rid is a sub-region of r and contains ptr and v, disjoint from each other
-  // - spine_rid is a sub-region of r, disjoint from ptr_v_rid, and contains the LL.footprint
+  // - spine_rid is a sub-region of r, disjoint from ptr_v_rid, and contains the LL1.footprint
   ST.is_eternal_region ll.r /\
   ST.is_eternal_region ll.spine_rid /\
   ST.is_eternal_region ll.ptr_v_rid /\
   B.(loc_includes (loc_region_only true ll.ptr_v_rid) (loc_addr_of_buffer ll.ptr `loc_union` loc_addr_of_buffer ll.v)) /\
-  B.(loc_includes (loc_region_only true ll.spine_rid) (LL.footprint h head v)) /\
+  B.(loc_includes (loc_region_only true ll.spine_rid) (LL1.footprint h head v)) /\
   B.(loc_disjoint (loc_addr_of_buffer ll.ptr) (loc_addr_of_buffer ll.v)) /\
   B.(loc_disjoint (loc_region_only true ll.ptr_v_rid) (loc_region_only true ll.spine_rid)) /\
 
@@ -77,12 +78,18 @@ val footprint: #a:Type -> h:HS.mem -> ll: t a -> Ghost B.loc
 let footprint #a h ll =
   let head = B.deref h ll.ptr in
   let v = B.deref h ll.v in
-  B.(loc_addr_of_buffer ll.ptr `loc_union` loc_addr_of_buffer ll.v `loc_union` LL.footprint h head v)
+  B.(loc_addr_of_buffer ll.ptr `loc_union` loc_addr_of_buffer ll.v `loc_union` LL1.footprint h head v)
 
 /// There! Much easier reasoning for clients.
 val v: #a:Type -> h:HS.mem -> ll: t a -> GTot (list a)
 let v #_ h ll =
   B.deref h ll.v
+
+val cells: #a:Type -> h:HS.mem -> ll: t a -> Ghost (list (B.pointer (LL1.cell a)))
+  (requires invariant h ll)
+  (ensures fun _ -> True)
+let cells #a h ll =
+  LL1.cells h (B.deref h ll.ptr) (B.deref h ll.v)
 
 // A workaround to avoid putting loc_all_regions_from true in patterns.
 let region_of ll = B.loc_all_regions_from false ll.r
@@ -101,7 +108,7 @@ let footprint_in_r #a (h: HS.mem) (ll: t a): Lemma
   (ensures B.(loc_includes (region_of ll) (footprint h ll)))
   //[ SMTPat (region_of ll); SMTPat (footprint h ll) ]
 =
-  assert B.(loc_includes (loc_region_only true ll.spine_rid) (LL.footprint h (B.deref h ll.ptr) (v h ll)));
+  assert B.(loc_includes (loc_region_only true ll.spine_rid) (LL1.footprint h (B.deref h ll.ptr) (v h ll)));
   assert B.(loc_includes (loc_all_regions_from true ll.r) (loc_region_only true ll.spine_rid))
 
 /// This lemma is perhaps overly precise, but for clients, as long as they know
@@ -146,7 +153,7 @@ val create_in: #a:Type -> r:HS.rid -> ST (t a)
 let create_in #a r =
   let ptr_v_rid = ST.new_region r in
   let spine_rid = ST.new_region r in
-  let ptr = B.malloc ptr_v_rid (B.null <: LL.t a) 1ul in
+  let ptr = B.malloc ptr_v_rid (B.null <: LL1.t a) 1ul in
   let v = B.malloc ptr_v_rid (G.hide ([] <: list a)) 1ul in
   { ptr; v; r; ptr_v_rid; spine_rid }
 #pop-options
@@ -164,7 +171,7 @@ val push: #a:Type -> ll: t a -> x: a -> ST unit
     v h1 ll == x :: v h0 ll)
 
 let push #a ll x =
-  LL.push ll.spine_rid (!* ll.v) ll.ptr x;
+  LL1.push ll.spine_rid (!* ll.v) ll.ptr x;
   let v = !* ll.v in
   ll.v *= G.hide (x :: v)
 
@@ -181,7 +188,7 @@ val pop: #a:Type -> ll: t a -> ST a
     x == hd)
 
 let pop #a ll =
-  let r = LL.pop ll.spine_rid (!* ll.v) ll.ptr in
+  let r = LL1.pop ll.spine_rid (!* ll.v) ll.ptr in
   let v = !* ll.v in
   ll.v *= G.hide (List.Tot.tl v);
   r
@@ -206,7 +213,7 @@ val maybe_pop: #a:Type -> ll: t a -> ST (option a)
 let maybe_pop #a ll =
   if not (B.is_null (!* ll.ptr)) then
     let v = !* ll.v in
-    let r = LL.pop ll.spine_rid (!* ll.v) ll.ptr in
+    let r = LL1.pop ll.spine_rid (!* ll.v) ll.ptr in
     ll.v *= G.hide (List.Tot.tl v);
     Some r
   else
@@ -224,7 +231,7 @@ val clear: #a:Type -> ll: t a -> ST unit
 
 let clear #a ll =
   let v = !* ll.v in
-  LL.free #_ #v ll.ptr;
+  LL1.free #_ #v ll.ptr;
   ll.v *= G.hide []
 
 val free: #a:Type -> ll: t a -> ST unit
@@ -235,7 +242,7 @@ val free: #a:Type -> ll: t a -> ST unit
 
 let free #_ ll =
   let v = !* ll.v in
-  LL.free #_ #v ll.ptr;
+  LL1.free #_ #v ll.ptr;
   B.free ll.ptr;
   B.free ll.v
 
